Sealing (WIP): Add [is_sealed] for sealing in verified code.

theories/heap_lang/lib/sealing.v
@@ -1,18 +1,32 @@
+From iris.algebra Require Import auth gmap agree.
+From iris.heap_lang Require Import addenda.
 From iris.heap_lang Require Export heap.
 From iris.heap_lang.lib Require Import abort lock maps.
 From iris.heap_lang Require Import notation proofmode.
+Import addenda.option.
 Import uPred.
 
 Local Notation ext R := (pointwise_relation _ R).
 
 (** * Dynamic sealing interface *)
 (**
-	Dynamic sealing offers protection analogous to the static
-	guarantees obtained with abstract types.
+	Morris introduced dynamic sealing in
+<<
+	James H. Morris Jr. Protection in Programming Languages.
+	CACM 16(1) (January 1973), 15–21.
+>>
+	His idea was to associate dynamic "type tags" with values
+	satisfying a representation invariant in order to approximate
+	the convenience of working in a language with abstract types
+	(while interoperating with untrusted, potentially ill-typed
+	code).
 
 	Our spec lets one pick a representation invariant [φ] when
 	allocating a sealer-unsealer pair. The [seal] and [unseal]
-	operations then convert between [φ] and [lowval].
+	operations then convert between [φ] and [lowval]. There are
+	two triples for [unseal]. The progressive triple returns a
+	predictable value, and is suitable for use in verified code.
+	The non-progressive triple returns *some* value.
 *)
 Module Import intf.
 
@@ -29,27 +43,33 @@ Section spec.
   Implicit Types v f : val.
 
   Structure sealing := Sealing {
-    (** Predicates. Name separates distinct instances. *)
+    (** Predicates. *)
+    (** Name separates ties [is_sealer_unsealer] to [is_sealed]. *)
     name : Type;
     is_sealer_unsealer (N : namespace) (γ : name) (v : val)
-      (φ : val → iProp Σ): iProp Σ;
+      (φ : val → iProp Σ) : iProp Σ;
+    is_sealed (N : namespace) (γ : name) (v v' : val) : iProp Σ;
     (** Structure *)
     is_sealer_unsealer_persistent N γ v φ :
       PersistentP (is_sealer_unsealer N γ v φ);
     is_sealer_unsealer_ne N γ v n :
       Proper (ext (dist n) ==> dist n) (is_sealer_unsealer N γ v);
-    is_sealer_unsealer_proper N γ v :
-      Proper (ext (≡) ==> (≡)) (is_sealer_unsealer N γ v);
+    is_sealed_persistent N γ v v' :
+      PersistentP (is_sealed N γ v v');
     (** Operations *)
     make_sealer_unsealer_spec N p φ `{Hφ : ∀ v, PersistentP (φ v)} :
       heapN ⊥ N →
       {{{ heap_ctx }}} make_sealer_unsealer SI () @ p; ⊤
       {{{ v γ, RET v; is_sealer_unsealer N γ v φ }}};
     seal_spec N p γ s φ `{Hφ : ∀ v, PersistentP (φ v)} :
-      {{{ is_sealer_unsealer N γ s φ }}} seal SI s @ p; ⊤ {{{ f, RET f;
-        ∀ p v, {{{ φ v }}} f v @ p; ⊤ {{{ v', RET v'; low v' }}}
+      {{{ is_sealer_unsealer N γ s φ }}} seal SI s @ p; ⊤ {{{ f, RET f; ∀ p v,
+        {{{ φ v }}} f v @ p; ⊤ {{{ v', RET v'; low v' ∗ is_sealed N γ v v' }}}
       }}};
-    unseal_spec N p γ s φ :
+    unseal_sealed_spec N p γ s φ :
+      {{{ is_sealer_unsealer N γ s φ }}} unseal SI s @ p; ⊤ {{{ f, RET f;
+        ∀ p v v', {{{ is_sealed N γ v v' }}} f v' @ p; ⊤ {{{ RET v; φ v }}}
+      }}};
+    unseal_low_spec N p γ s φ :
       {{{ is_sealer_unsealer N γ s φ }}} unseal SI s @ p; ⊤ {{{ f, RET f;
         ∀ v', {{{ low v' }}} f v' ?{{{ v, RET v; φ v }}}
       }}}
@@ -57,15 +77,22 @@ Section spec.
 End spec.
 Arguments sealing _ {_ _}.
 Existing Instances is_sealer_unsealer_persistent is_sealer_unsealer_ne
-  is_sealer_unsealer_proper.
+  is_sealed_persistent.
 
 Section lemmas.
   Context `{heapG Σ, SI : SealingImpl} (S : sealing Σ).
   Implicit Types v : val.
 
+  Global Instance is_sealer_unsealer_proper N γ v :
+    Proper (ext (≡) ==> (≡)) (is_sealer_unsealer S N γ v).
+  Proof.
+    move=>???. apply equiv_dist=>?. apply is_sealer_unsealer_ne=>?.
+    by apply equiv_dist.
+  Qed.
+
   Lemma seal_val N p γ s φ v `{Hφ : ∀ v, PersistentP (φ v)} :
     {{{ is_sealer_unsealer S N γ s φ ∗ φ v }}} seal SI s v @ p; ⊤
-    {{{ v', RET v'; low v' }}}.
+    {{{ v', RET v'; low v' ∗ is_sealed S N γ v v' }}}.
   Proof.
     iIntros (Φ) "#[Hs Hv] HΦ".
     wp_apply (seal_spec with "Hs"). iIntros (f) "Hf".
@@ -73,12 +100,22 @@ Section lemmas.
     by iApply ("HΦ" with "Hv'").
   Qed.
 
-  Lemma unseal_val N γ s φ v' :
+  Lemma unseal_sealed_val N p γ s φ v v' :
+    {{{ is_sealer_unsealer S N γ s φ ∗ is_sealed S N γ v v' }}}
+      unseal SI s v' @ p; ⊤
+    {{{ RET v; φ v }}}.
+  Proof.
+    iIntros (Φ) "#[Hs Hv'] HΦ".
+    wp_apply (unseal_sealed_spec with "Hs"). iIntros (f) "Hf".
+    by wp_apply ("Hf" with "* Hv'").
+  Qed.
+
+  Lemma unseal_low_val N γ s φ v' :
     {{{ is_sealer_unsealer S N γ s φ ∗ low v' }}} unseal SI s v'
     ?{{{ v, RET v; φ v }}}.
   Proof.
     iIntros (Φ) "#[Hs Hv'] HΦ".
-    wp_apply (unseal_spec with "Hs"). iIntros (f) "Hf".
+    wp_apply (unseal_low_spec with "Hs"). iIntros (f) "Hf".
     by wp_apply ("Hf" with "* Hv'").
   Qed.
 End lemmas.
@@ -86,17 +123,12 @@ End intf.
 
 (** * Morris' dynamic sealing implementation *)
 (**
-	Adpated from
-<<
-		James H. Morris Jr. Protection in Programming
-		Languages. CACM 16(1) (January 1973), 15–21.
->>
 	Safe-for-space implementations exist. The sequential code
 <<
-		let r = ref None in
-		let seal x = λ _, r := Some x in
-		let unseal f = (r := None; f (); valOf (! r)) in
-		(seal, unseal)
+	let r = ref None in
+	let seal x = λ _, r := Some x in
+	let unseal f = (r := None; f (); valOf (! r)) in
+	(seal, unseal)
 >>
 	could be adpated to the concurrent setting (e.g., using
 	reentrant locks).
@@ -104,7 +136,7 @@ End intf.
 	Attribution: This sequential implementation isn't new. It is
 	based on E language code at
 <<
-		http://wiki.erights.org/wiki/Walnut/Secure_Distributed_Computing/Capability_Patterns#Sealers_and_Unsealers
+	http://wiki.erights.org/wiki/Walnut/Secure_Distributed_Computing/Capability_Patterns#Sealers_and_Unsealers
 >>
 	(accessed in February 2017).
 *)
@@ -132,123 +164,304 @@ End code.
 
 Definition sealing (LI : LockImpl) : SealingImpl := {|
   intf.make_sealer_unsealer := make_sealer_unsealer LI;
-  intf.seal := seal;
-  intf.unseal := unseal
+  intf.seal := seal; intf.unseal := unseal
 |}.
 End code.
 
 Module proof.
+(** The CMRA we need. *)
+Notation heap := (gmap loc val).
+Definition heapUR : ucmraT := gmapUR loc (agreeR valC).
+Class sealingG Σ := SealingG { sealing_heapG :> inG Σ (authR heapUR) }.
+
+Definition sealingΣ : gFunctors := #[ GFunctor (constRF (authR heapUR)) ].
+Instance subG_sealingΣ {Σ} : subG sealingΣ Σ → sealingG Σ.
+Proof. intros [??]%subG_inv. constructor; apply _. Qed.
+
 Section proof.
-  Context `{heapG Σ, LI : LockImpl} (L : lock Σ) (N : namespace).
+  Context `{heapG Σ, sealingG Σ, LI : LockImpl} (L : lock Σ) (N : namespace).
   Let SI : SealingImpl := code.sealing LI.
   Implicit Types l : loc.
   Implicit Types f v : val.
   Notation ext R := (pointwise_relation _ R).
 
-  Definition tbl_res (l : loc) (φ : val → iProp Σ) : iProp Σ := (
-    ∃ map m, l ↦ map ∗ is_map (K:=loc) map m ∗ □ [∗ map] v ∈ m, φ v
+  Let name : Type := gname * loc.
+
+  (**
+	The assertion [is_witness γ k v] represents knowledge that the
+	table underlying the sealer-unsealer pair named [γ] sends
+	location [k] to value [v].
+  *)
+  Definition is_witness (γ : name) (k : loc) (v : val) : iProp Σ :=
+    own (γ.1) (◯ {[k := to_agree v]}).
+
+  (**
+	The table underlying the sealer-unsealer pair named [γ] sends
+	locations [k] to values satisfying the representation
+	invariant [φ]. Moreover, locations [k] arising from verified
+	applications of [unseal] are tied to a ghost heap witnessing
+	the table's assignment of a particular value [v] to [k].
+
+	The table can bind locations not tracked by the ghost heap
+	because adversarial code can apply a sealed value to a
+	low-integrity value [kv]. When [kv] is a location [k], such
+	applications extend the table (but not the ghost heap).
+
+	We store actual heap resources alongside the ghost heap to
+	ensure we can allocate [is_witness γ k v] given a fresh, high
+	location [k].
+  *)
+  Definition to_heap : heap → heapUR := fmap to_agree.
+
+  Definition witness (γ : name) (m : heap) : iProp Σ := (
+    ∃ h, ⌜h ⊆ m⌝ ∗ own (γ.1) (● to_heap h) ∗ live (dom _ h) ∗
+    [∗ map] k↦_ ∈ h, k ↦ ()
   )%I.
 
-  Definition is_sealer_unsealer (l : loc) (v : val) (φ : val → iProp Σ) : iProp Σ := (
-    ∃ sync, ⌜heapN ⊥ N⌝ ∗ heap_ctx ∗ ⌜v = (sync, l)%V⌝ ∗
-    is_sync sync (tbl_res l φ)
+  Definition tbl_res (γ : name) (φ : val → iProp Σ) : iProp Σ := (
+    ∃ map m, (γ.2) ↦ map ∗ is_map map m ∗ witness γ m ∗
+    [∗ map] v ∈ m, □ φ v
   )%I.
 
-  Global Instance is_sealer_unsealer_persistent l v φ :
-    PersistentP (is_sealer_unsealer l v φ).
+  Definition is_sealer_unsealer (γ : name) (v : val) φ : iProp Σ := (
+    ∃ sync, ⌜heapN ⊥ N⌝ ∗ heap_ctx ∗ ⌜v = (sync, γ.2)%V⌝ ∗
+    is_sync sync (tbl_res γ φ)
+  )%I.
+
+  (*
+	The assertion [is_sealed γ v v'] represents knowledge that
+	value [v'] was obtained by sealing value [v] with the
+	sealer-unsealer pair named [γ].
+
+	Unfolding the definition, we have a progressive triple for [v'
+	k] that converts a high, fresh location [k] to a witness
+	[is_witness γ k v] sufficient to ensure that table lookups on
+	[k] will compute [v]
+  *)
+  Definition is_sealed (γ : name) (v v' : val) : iProp Σ := (
+    ∀ p k,
+    {{{ k ↦ () ∗ fresh k }}} v' k @ p; ⊤ {{{ RET (); is_witness γ k v }}}
+  )%I.
+
+  (** Structure *)
+
+  Instance is_witness_persistent γ k v : PersistentP (is_witness γ k v).
+  Proof. apply _. Qed.
+  Instance is_witness_timeless γ k v : TimelessP (is_witness γ k v).
   Proof. apply _. Qed.
 
-  Instance tbl_res_ne l n : Proper (ext (dist n) ==> dist n) (tbl_res l).
+  Instance tbl_res_ne γ n : Proper (ext (dist n) ==> dist n) (tbl_res γ).
   Proof. solve_proper. Qed.
 
-  Global Instance is_sealer_unsealer_ne l v n :
-    Proper (ext (dist n) ==> dist n) (is_sealer_unsealer l v).
-  Proof. solve_proper. Qed.
+  Global Instance is_sealer_unsealer_persistent γ v φ :
+    PersistentP (is_sealer_unsealer γ v φ).
+  Proof. apply _. Qed.
+  Global Instance is_sealer_unsealer_ne γ v n :
+    Proper (ext (dist n) ==> dist n) (is_sealer_unsealer γ v).
+  Proof.
+    (* FIXME: [solve_proper] works but is very slow here *)
+    move=>φ1 φ2 Hφ. preprocess_solve_proper.
+    apply exist_ne. do 4!f_equiv. apply is_sync_ne. f_equiv. by apply Hφ.
+  Qed.
 
-  Instance tbl_res_proper l : Proper (ext (≡) ==> (≡)) (tbl_res l).
-  Proof. solve_proper. Qed.
+  Global Instance is_sealed_persistent γ v v' : PersistentP (is_sealed γ v v').
+  Proof. apply _. Qed.
 
-  Global Instance is_sealer_unsealer_proper l v :
-    Proper (ext (≡) ==> (≡)) (is_sealer_unsealer l v).
-  Proof. solve_proper. Qed.
+  (** Ghosts *)
 
+  Lemma witness_elim γ m k v :
+    witness γ m -∗ is_witness γ k v -∗ ⌜m !! k = Some v⌝.
+  Proof.
+    iIntros "Hw Hk". iDestruct "Hw" as (h) "(%&Hγ&_)".
+    iDestruct (own_valid_2 with "Hγ Hk") as %[Hinc _]%auth_valid_discrete_2.
+    iPureIntro. apply (map_subseteq_spec h m); first done.
+    move: Hinc. rewrite singleton_included lookup_fmap=>-[] u [].
+    case: (h !! k)=>[vh|]/=; last by move=>/option_equivE.
+    move=>Heq. apply (inj Some) in Heq. unfold_leibniz. rewrite -Heq.
+    by case/Some_included=>[/(inj to_agree) | /to_agree_included]->.
+  Qed.
+
+  Lemma witness_high_alloc γ h k v :
+    h !! k = None →
+    own (γ.1) (● to_heap h) ==∗
+    own (γ.1) (● to_heap (<[k:=v]> h)) ∗ is_witness γ k v.
+  Proof.
+    rewrite /to_heap fmap_insert -own_op=>Hdom.
+    apply own_update, auth_update_alloc, alloc_singleton_local_update.
+    by rewrite lookup_fmap Hdom. done.
+  Qed.
+
+  Lemma witness_high γ m k v :
+    heap_ctx -∗ witness γ m -∗ k ↦ () -∗ fresh k ={⊤}=∗
+    witness γ (<[k:=v]> m) ∗ is_witness γ k v.
+  Proof.
+    iIntros "#Hh Hw Hk Hf". iDestruct "Hw" as (h) "(%&Hγ&Hlive&Hhigh)".
+    iMod (heap_mark_live with "Hh Hf Hlive") as "(Hdom&Hlive)"; first done.
+      iDestruct "Hdom" as %?%not_elem_of_dom.
+    iMod (witness_high_alloc _ _ k v with "Hγ") as "[Hγ Hw]"; first done.
+    iModIntro. iFrame "Hw". iExists (<[k:=v]> h). iFrame "Hγ".
+    rewrite dom_insert_L. iFrame "Hlive".
+    rewrite big_sepM_insert //. iFrame "Hk Hhigh".
+    iPureIntro. apply map_subseteq_spec=>x vx.
+    case: (decide (k = x))=>[<-|?]; first by rewrite !lookup_insert.
+    do 2!rewrite lookup_insert_ne //. by apply (map_subseteq_spec h m).
+  Qed.
+
+  Lemma witness_low_sep (h : heap) k :
+    ([∗ map] k↦_ ∈ h, k ↦ ()) -∗ low k -∗ ⌜h !! k = None⌝.
+  Proof.
+    induction h as [|x vx h Hx IH] using map_ind; iIntros "Hhigh Hl";
+      first by rewrite lookup_empty.
+    rewrite big_sepM_insert //. iDestruct "Hhigh" as "[Hh Hhigh]".
+    case: (decide (k = x))=>?.
+    - iExFalso. subst. by iApply (high_not_low with "[$Hh $Hl]").
+    - rewrite lookup_insert_ne //. by iApply (IH with "Hhigh Hl").
+  Qed.
+
+  Lemma witness_low γ m k v :
+    witness γ m -∗ low k -∗ witness γ (<[k:=v]> m).
+  Proof.
+    iIntros "Hw Hk". iDestruct "Hw" as (h) "(%&Hγ&Hlive&Hhigh)". iExists h.
+    iDestruct (witness_low_sep with "Hhigh Hk") as "#Hdom".
+      iDestruct "Hdom" as %Hdom.
+    iFrame "Hγ Hlive Hhigh". iPureIntro. apply map_subseteq_spec=>x vx.
+    case: (decide (k = x))=>[<-|?]; first by rewrite Hdom.
+    rewrite lookup_insert_ne //. by apply map_subseteq_spec.
+  Qed.
+
+  Lemma tbl_inv_insert (m : heap) k v (φ : val → iProp Σ)
+      `{Hv : ∀ v, PersistentP (φ v)} :
+    ([∗ map] v ∈ m, □ φ v) -∗ φ v -∗ [∗ map] v ∈ <[k:=v]> m, □ φ v.
+  Proof.
+    iIntros "Hinv #Hv". case Hv': (m !! k) => [v'|].
+    - rewrite (big_sepM_insert_override_2 _ _ _ v' v) //.
+      iApply "Hinv". iIntros "_". iAlways. by iFrame "Hv".
+    - rewrite big_sepM_insert //. iFrame "Hinv". iAlways. by iFrame "Hv".
+  Qed.
+
+  (** Operations *)
+
+(* PDS: We probably do not need heapN ⊥ N after allocation. *)
   Lemma make_sealer_unsealer_spec p φ `{Hφ : ∀ v, PersistentP (φ v)} :
     heapN ⊥ N →
     {{{ heap_ctx }}} make_sealer_unsealer SI () @ p; ⊤
-    {{{ v l, RET v; is_sealer_unsealer l v φ }}}.
+    {{{ v γ, RET v; is_sealer_unsealer γ v φ }}}.
   Proof.
     iIntros (? Φ) "#Hh HΦ". wp_lam. wp_alloc l as "Hl". wp_let.
-    wp_apply (make_sync_spec L _ N (tbl_res l φ) with "[$Hh Hl]")=>//.
-    { iExists map_empty, ∅. iFrame "Hl". iSplitL; auto. iAlways.
-      by rewrite big_sepM_empty. }
+      rewrite -wp_fupd. set h := to_heap ∅.
+    iMod (own_alloc (Auth (Excl' h) h)) as (γh) "Hγh"; first done.
+      rewrite (auth_both_op h). iDestruct "Hγh" as "[Hγh _]".
+      set γ : name := (γh, l).
+    iAssert (witness γ ∅) with "[Hγh]" as "Hw".
+    { iExists ∅. iFrame "Hγh".
+      rewrite dom_empty_L big_sepS_empty big_sepM_empty. by auto. }
+    wp_apply (make_sync_spec L _ N (tbl_res γ φ) with "[$Hh Hl Hw]");
+      first done.
+    { iExists map_empty, ∅. iFrame "Hl Hw". rewrite big_sepM_empty. by auto. }
     iIntros (sync) "Hsync". wp_let.
-    iApply "HΦ". iExists sync. by iFrame "% Hh Hsync".
+    iApply ("HΦ" $! _ γ). iExists sync. by iFrame "% Hh Hsync".
   Qed.
 
-  Lemma seal_spec p l s φ `{Hφ : ∀ v, PersistentP (φ v)} :
-    {{{ is_sealer_unsealer l s φ }}} seal SI s @ p; ⊤ {{{ f, RET f;
-      ∀ p v, {{{ φ v }}} f v @ p; ⊤ {{{ v', RET v'; low v' }}}
+  Lemma seal_spec p γ s φ `{Hφ : ∀ v, PersistentP (φ v)} :
+    {{{ is_sealer_unsealer γ s φ }}} seal SI s @ p; ⊤ {{{ f, RET f; ∀ p v,
+      {{{ φ v }}} f v @ p; ⊤ {{{ v', RET v'; low v' ∗ is_sealed γ v v' }}}
     }}}.
   Proof.
     iIntros (Φ) "#Hs HΦ". wp_lam.
     iApply "HΦ". clear p Φ. iIntros (p v) "!#". iIntros (Φ) "#Hv HΦ". wp_lam.
-    iApply "HΦ". clear Φ. rewrite low_rec. iAlways. iNext.
-      iIntros (vk Φ) "_ HΦ". simpl_subst.
-      iDestruct "Hs" as (sync) "(%&#Hh&%&Hsync)". subst.
-      do 2!(wp_proj; wp_let).
-    wp_typecast Hloc; wp_match; last by wp_apply wp_abort.
-      destruct (is_loc_val _ Hloc) as (k&->). rewrite/is_sync.
-    wp_apply ("Hsync" with "[%]"). iClear "Hsync". iIntros (Ψ) "HR HΨ".
-      iDestruct "HR" as (map m) "(Hl & Hm & #Hrng)". wp_load.
-    (* PDS: Hack. *)
-      iDestruct (map_insert_spec map noprogress ⊤ m k v with "Hm") as "Hins".
-      rewrite /map_insert.
-    wp_apply "Hins". iIntros (map') "Hm'". wp_store.
-    iApply ("HΨ" with "[Hl Hm']"); last by iApply "HΦ"; simpl_low.
-    iExists map', (<[k:=v]> m). iFrame "Hl Hm'". iAlways.
-    case Hv': (m !! k) => [v'|].
-    - rewrite (big_sepM_insert_override_2 _ _ _ v' v) //.
-      iApply "Hrng". by iIntros.
-    - rewrite big_sepM_insert //. by iFrame "Hv Hrng".
+    iApply "HΦ". clear Φ. iSplitL.
+
+    (** The seal is a low function. *)
+    - rewrite low_rec. iAlways. iNext. iIntros (vk Φ) "#Hk HΦ". simpl_subst.
+        iDestruct "Hs" as (sync) "(%&#Hh&%&Hsync)". subst.
+        do 2!(wp_proj; wp_let).
+      wp_typecast Hloc; wp_match; last by wp_apply wp_abort.
+        destruct (is_loc_val _ Hloc) as (k&->). rewrite/is_sync.
+      wp_apply ("Hsync" with "[%]"). iClear "Hsync". iIntros (Ψ) "HR HΨ".
+        iDestruct "HR" as (map m) "(Hl & Hm & Hw & #Hinv)". wp_load.
+      wp_apply (map_insert_spec _ _ _ m with "Hm").
+        iIntros (map') "Hm'". wp_store.
+      iApply ("HΨ" with "[Hl Hm' Hw]"); last by iApply "HΦ"; simpl_low.
+      iExists map', (<[k:=v]> m). iFrame "Hl Hm'". iSplitL.
+      + rewrite (low_val k). by iApply (witness_low with "Hw Hk").
+      + by iApply (tbl_inv_insert with "Hinv Hv").
+
+    (** The seal satisfies [is_sealed]. *)
+    - clear p. iIntros (p k) "!#". iIntros (Φ) "[Hk Hf] HΦ". wp_lam.
+        iDestruct "Hs" as (sync) "(%&#Hh&%&Hsync)". subst.
+        do 2!(wp_proj; wp_let).
+      wp_typecast Hloc; last by exfalso; apply Hloc; exists k.
+        wp_match. rewrite/is_sync.
+      wp_apply ("Hsync" with "[%]"). iClear "Hsync". iIntros (Ψ) "HR HΨ".
+        iDestruct "HR" as (map m) "(Hl & Hm & Hw & #Hinv)". wp_load.
+      wp_apply (map_insert_spec _ _ _ m with "Hm").
+        iIntros (map') "Hm'". rewrite -wp_fupd. wp_store.
+      iMod (witness_high _ _ k v with "Hh Hw Hk Hf") as "[Hw Hkv]".
+      iApply ("HΨ" with "[Hl Hm' Hw]"); last by iApply ("HΦ" with "Hkv").
+      iExists map', (<[k:=v]> m). iFrame "Hl Hm' Hw".
+      by iApply (tbl_inv_insert with "Hinv Hv").
   Qed.
 
-  Lemma unseal_spec p l s φ :
-    {{{ is_sealer_unsealer l s φ }}} unseal SI s @ p; ⊤ {{{ f, RET f;
+  Lemma unseal_sealed_spec p γ s φ :
+    {{{ is_sealer_unsealer γ s φ }}} unseal SI s @ p; ⊤ {{{ f, RET f;
+      ∀ p v v', {{{ is_sealed γ v v' }}} f v' @ p; ⊤ {{{ RET v; φ v }}}
+    }}}.
+  Proof.
+    iIntros (Φ) "#Hs HΦ". wp_lam.
+    iApply "HΦ". clear p Φ. iIntros (p v v') "!#". iIntros (Φ) "#Hv' HΦ".
+      wp_lam. iDestruct "Hs" as (sync) "(%&#Hh&%&Hsync)". subst.
+      do 2!(wp_proj; wp_let).
+    wp_apply (wp_alloc_fresh with "Hh"); auto.
+      iIntros (k) "[Hk Hf]". wp_let. rewrite/is_sealed.
+    wp_apply ("Hv'" with "* [$Hk $Hf]"). iIntros "Hkv". wp_seq. rewrite/is_sync.
+    wp_apply ("Hsync" with "[%]"). iClear "Hsync". iIntros (Ψ) "HR HΨ".
+      iDestruct "HR" as (map m) "(Hl & #Hm & Hw & #Hinv)". wp_load.
+      iDestruct (witness_elim with "Hw Hkv") as "%".
+    wp_apply (map_lookup_partial_Some_spec _ _ _ _ k with "Hm");
+      first done. iIntros "_".
+    iApply ("HΨ" with "[Hl Hw]").
+    - iExists map, m. by iFrame "Hl Hm Hw Hinv".
+    - iApply "HΦ". setoid_rewrite always_elim.
+      by iApply (big_sepM_lookup (λ _, φ) m k v with "Hinv").
+  Qed.
+
+  Lemma unseal_low_spec p γ s φ :
+    {{{ is_sealer_unsealer γ s φ }}} unseal SI s @ p; ⊤ {{{ f, RET f;
       ∀ v', {{{ low v' }}} f v' ?{{{ v, RET v; φ v }}}
     }}}.
   Proof.
     iIntros (Φ) "#Hs HΦ". wp_lam.
     iApply "HΦ". clear Φ. iIntros (v') "!#". iIntros (Φ) "#Hv' HΦ". wp_lam.
-      iDestruct "Hs" as (sync) "(%&#Hh&%&Hsync)". subst.
-      do 2!(wp_proj; wp_let).
+      iDestruct "Hs" as (sync) "(%&#Hh&%&Hsync)". subst. do 2!(wp_proj; wp_let).
     wp_apply (wp_alloc_low with "[$Hh]"); auto; first by simpl_low.
       iIntros (k) "Hk". wp_let.
-    (* PDS: Hack. *)
-    (*
-	[wp_on_val_app] should be a Texan triple.
-	And, once we simplify robust safety, there's no call for
-	stating those lemmas in terms of expression.
-    *)
+(*
+	PDS: Hack. [wp_on_val_app] should be a Texan triple and
+	there's no call to state those lemmas in terms of expressions.
+*)
     wp_bind (v' k). iDestruct (wp_on_val_app lowloc v' k) as "Happ".
       rewrite (wp_wand _ _ (v' k)%E _ _).
     wp_apply ("Happ" with "[Hv'] [Hk]");
       [by rewrite low_val_eq|by rewrite low_loc on_val_elim|].
     iIntros (?) "_". wp_seq. iClear "Happ".
-    (* PDS: End hack. *)
+(* PDS: End hack. *)
     rewrite/is_sync.
-    wp_apply ("Hsync" with "[%]"). iIntros (Ψ) "HR HΨ".
-      iDestruct "HR" as (map m) "(Hl & #Hm & #Hrng)". wp_load.
+    wp_apply ("Hsync" with "[%]"). iClear "Hsync". iIntros (Ψ) "HR HΨ".
+      iDestruct "HR" as (map m) "(Hl & #Hm & Hw & #Hinv)". wp_load.
     wp_apply (map_lookup_partial_spec _ _  _ k with "Hm")=>//.
       iIntros (v'') "%".
-    iApply ("HΨ" with "[Hl]").
-    - iExists map, m. iFrame "Hl Hm". iAlways. by iFrame "Hrng".
-    - iApply "HΦ". by rewrite -(big_sepM_lookup (λ k v, φ v) m k v'').
+    iApply ("HΨ" with "[Hl Hw]").
+    - iExists map, m. by iFrame "Hl Hm Hw Hinv".
+    - iApply "HΦ". setoid_rewrite always_elim.
+      by rewrite -(big_sepM_lookup (λ _, φ) m k v'').
   Qed.
 End proof.
 
-Definition sealing `{heapG Σ, LockImpl} (L : lock Σ) : sealing Σ := {|
+Definition sealing `{heapG Σ, sealingG Σ, LockImpl}
+    (L : lock Σ) : sealing Σ := {|
   intf.make_sealer_unsealer_spec := make_sealer_unsealer_spec L;
   intf.seal_spec := seal_spec;
-  intf.unseal_spec := unseal_spec
+  intf.unseal_sealed_spec := unseal_sealed_spec;
+  intf.unseal_low_spec := unseal_low_spec
 |}.
 End proof.
